src/Index.v
@@ -1,0 +1,146 @@
+Require Import Bool Ascii List Omega.
+Require Import Common.
+
+Local Open Scope list.
+
+Definition IdxT := list nat.
+
+Definition natToIdx (n: nat): IdxT := n :: nil.
+Coercion natToIdx: nat >-> IdxT.
+
+Definition idx_dec: forall (idx1 idx2: IdxT), {idx1 = idx2} + {idx1 <> idx2}.
+Proof.
+  intros.
+  decide equality.
+  apply eq_nat_dec.
+Defined.
+
+Fixpoint idx_lt (idx1 idx2: IdxT): Prop :=
+  match idx1 with
+  | nil => match idx2 with
+           | nil => False
+           | _ => True
+           end
+  | e1 :: t1 =>
+    match idx2 with
+    | nil => False
+    | e2 :: t2 =>
+      if lt_dec e1 e2 then True
+      else if lt_dec e2 e1 then False
+           else idx_lt t1 t2
+    end
+  end.
+
+Fixpoint idx_lt_dec (idx1 idx2: IdxT): {idx_lt idx1 idx2} + {~ idx_lt idx1 idx2}.
+Proof.
+  destruct idx1.
+  - destruct idx2.
+    + right; auto.
+    + left; simpl; auto.
+  - destruct idx2.
+    + right; auto.
+    + simpl.
+      destruct (lt_dec n n0); auto.
+      destruct (lt_dec n0 n); auto.
+Defined.
+
+Definition idx_total:
+  forall idx1 idx2, idx1 <> idx2 -> idx_lt idx1 idx2 \/ idx_lt idx2 idx1.
+Proof.
+  induction idx1 as [|n1 idx1]; simpl; intros;
+    [destruct idx2; [exfalso; auto|auto]|].
+
+  destruct idx2 as [|n2 idx2]; [right; simpl; auto|].
+  simpl; destruct (lt_dec n2 n1); [right; simpl; auto|].
+  pose proof (Nat.lt_total n2 n1) as Ht.
+  destruct Ht as [|[|]].
+  - exfalso; auto.
+  - subst.
+    destruct (lt_dec n1 n1); [exfalso; omega|clear n0].
+    apply IHidx1.
+    intro Hx; subst; auto.
+  - destruct (lt_dec n1 n2); auto.
+Qed.
+
+Definition idx_lt_trans:
+  forall idx1 idx2 idx3: IdxT,
+    idx_lt idx1 idx2 -> idx_lt idx2 idx3 -> idx_lt idx1 idx3.
+Proof.
+  induction idx1 as [|n1 idx1]; simpl; intros.
+  - destruct idx2 as [|n2 idx2]; [exfalso; auto|].
+    destruct idx3 as [|n3 idx3]; [inv H0|].
+    auto.
+  - destruct idx2 as [|n2 idx2]; [exfalso; auto|].
+    destruct idx3 as [|n3 idx3]; [inv H0|].
+    simpl in H0.
+    destruct (lt_dec n1 n2).
+    + destruct (lt_dec n2 n3).
+      * destruct (lt_dec n1 n3); auto.
+        exfalso; omega.
+      * destruct (lt_dec n3 n2); [exfalso; auto|].
+        destruct (lt_dec n1 n3); auto.
+        exfalso; omega.
+    + destruct (lt_dec n2 n3).
+      * destruct (lt_dec n2 n1); [exfalso; auto|].
+        destruct (lt_dec n1 n3); auto.
+        exfalso; omega.
+      * destruct (lt_dec n2 n1); [exfalso; auto|].
+        destruct (lt_dec n3 n2); [exfalso; auto|].
+        destruct (lt_dec n1 n3); auto.
+        destruct (lt_dec n3 n1); [omega|].
+        eapply IHidx1; eassumption.
+Qed.
+
+Definition idx_lt_not_eq:
+  forall idx1 idx2: IdxT, idx_lt idx1 idx2 -> idx1 <> idx2.
+Proof.
+  intros.
+  intro Hx; subst.
+  induction idx2 as [|n2 idx2]; [inv H|].
+  simpl in H.
+  destruct (lt_dec n2 n2); [omega|auto].
+Qed.
+
+Definition Id (A: Type) := (IdxT * A)%type.
+
+Definition idOf {A} (ida: Id A) := fst ida.
+Definition valOf {A} (ida: Id A) := snd ida.
+Definition idsOf {A} (ias: list (Id A)) := List.map fst ias.
+Definition valsOf {A} (ias: list (Id A)) := List.map snd ias.
+
+Definition liftI {A B: Type} (f: A -> B) (ida: Id A): Id B :=
+  (idOf ida, f (valOf ida)).
+
+Definition imap {A B: Type} (f: A -> B) (ias: list (Id A)): list (Id B) :=
+  List.map (liftI f) ias.
+Definition ifilterI {A} (ias: list (Id A)) (f: IdxT -> bool): list (Id A) :=
+  filter (fun ia => f (idOf ia)) ias.
+Definition ifilterV {A} (ias: list (Id A)) (f: A -> bool): list (Id A) :=
+  filter (fun ia => f (valOf ia)) ias.
+
+Definition id_dec {A} (a_dec: forall (a1 a2: A), {a1 = a2} + {a1 <> a2}):
+  forall (ida1 ida2: Id A), {ida1 = ida2} + {ida1 <> ida2}.
+Proof.
+  intros.
+  decide equality.
+  apply idx_dec.
+Defined.
+
+Definition extendIdx (ext: nat) (idx: IdxT): IdxT :=
+  ext :: idx.
+
+Definition extendInds (ext: nat) (inds: list IdxT): list IdxT :=
+  map (extendIdx ext) inds.
+
+Definition liftInds (ns: list nat): list IdxT :=
+  map natToIdx ns.
+
+Definition idxHd (idx: IdxT): nat :=
+  List.hd 0 idx.
+
+Fixpoint nat_seq_rev (n: nat) :=
+  match n with
+  | O => O :: nil
+  | S n' => n :: nat_seq_rev n'
+  end.
+
